HOTG/Cardinals/HOTG_Cardinals_Multiplication.thy
@@ -1,10 +1,12 @@
+\<^marker>\<open>creator "Niklas Krofta"\<close>
+\<^marker>\<open>creator "Kevin Kappelmann"\<close>
 theory HOTG_Cardinals_Multiplication
   imports HOTG_Cardinals_Base HOTG_Pairs
 begin
 
 unbundle no_HOL_groups_syntax
 
-definition "cardinal_mul \<kappa> \<mu> \<equiv> |\<kappa> \<times> \<mu>|"
+definition "cardinal_mul X Y \<equiv> |X \<times> Y|"
 
 bundle hotg_cardinal_mul_syntax begin notation cardinal_mul (infixl "\<otimes>" 65) end
 bundle no_hotg_cardinal_mul_syntax begin no_notation cardinal_mul (infixl "\<otimes>" 65) end
@@ -12,6 +14,28 @@ unbundle hotg_cardinal_mul_syntax
 
 lemma cardinal_mul_eq_cardinality_pair: "X \<otimes> Y = |X \<times> Y|"
   unfolding cardinal_mul_def ..
+
+lemma pair_equipollent_self_commute: "X \<times> Y \<approx> Y \<times> X"
+  by (intro equipollentI[where ?f=swap and ?g=swap]) (fastforce dest: inverse_onD)
+
+lemma cardinal_mul_comm: "X \<otimes> Y = Y \<otimes> X"
+  unfolding cardinal_mul_eq_cardinality_pair
+  by (intro cardinality_eq_if_equipollent pair_equipollent_self_commute)
+
+lemma empty_pair_equipollent_self: "{} \<times> X \<approx> {}"
+  by (intro equipollentI) fastforce
+
+corollary zero_cardinal_mul_eq_zero [simp]: "0 \<otimes> X = 0"
+  unfolding cardinal_mul_eq_cardinality_pair by (subst cardinality_zero_eq_zero[symmetric])
+  (intro cardinality_eq_if_equipollent empty_pair_equipollent_self)
+
+lemma pair_equipollent_assoc: "(X \<times> Y) \<times> Z \<approx> X \<times> (Y \<times> Z)"
+proof (rule equipollentI)
+   show "bijection_on ((X \<times> Y) \<times> Z :: set) (X \<times> (Y \<times> Z))
+      (\<lambda>\<langle>p, z\<rangle>. \<langle>fst p, \<langle>snd p, z\<rangle>\<rangle>)
+      (\<lambda>\<langle>x, p\<rangle>. \<langle>\<langle>x, fst p\<rangle>, snd p\<rangle>)"
+    by (urule (rr) bijection_onI dep_mono_wrt_predI inverse_onI) fastforce+
+qed
 
 lemma pair_equipollent_if_equipollent:
   assumes "X \<approx> X'" and "Y \<approx> Y'"
@@ -31,11 +55,22 @@ proof -
 qed
 
 corollary cardinality_pair_cardinality_equipollent_pair: "|X| \<times> |Y| \<approx> X \<times> Y"
-  using pair_equipollent_if_equipollent by auto
+  by (rule pair_equipollent_if_equipollent) simp_all
 
-corollary cardinality_cardinal_mul_eq_cardinality_pair: "|X| \<otimes> |Y| = |X \<times> Y|"
-  using cardinal_mul_eq_cardinality_pair cardinality_pair_cardinality_equipollent_pair
-    cardinality_eq_if_equipollent
-  by auto
+corollary cardinality_cardinal_mul_eq_cardinal_mul [simp]: "|X| \<otimes> |Y| = X \<otimes> Y"
+  unfolding cardinal_mul_eq_cardinality_pair
+  by (intro cardinality_eq_if_equipollent cardinality_pair_cardinality_equipollent_pair)
+
+lemma cardinal_mul_assoc: "(X \<otimes> Y) \<otimes> Z = X \<otimes> (Y \<otimes> Z)"
+proof -
+  have "|(X \<times> Y)| \<times> Z \<approx> (X \<times> Y) \<times> Z"
+    using reflexive_equipollent by (blast intro: pair_equipollent_if_equipollent dest: reflexiveD)
+  moreover have "... \<approx> X \<times> (Y \<times> Z)" by (simp add: pair_equipollent_assoc)
+  moreover have "... \<approx> X \<times> |Y \<times> Z|" using partial_equivalence_rel_equipollent
+    by (blast intro: pair_equipollent_if_equipollent dest: reflexiveD symmetricD)
+  ultimately have "|(X \<times> Y)| \<times> Z \<approx> X \<times> |Y \<times> Z|" using transitive_equipollent by blast
+  then show ?thesis
+    by (auto intro: cardinality_eq_if_equipollent simp: cardinal_mul_eq_cardinality_pair)
+qed
 
 end
