HOTG/Mem_Transitive_Closure/HOTG_Mem_Transitive_Closure.thy
@@ -4,7 +4,8 @@ section \<open>Transitive Closure With Respect To Membership\<close>
 theory HOTG_Mem_Transitive_Closure
   imports
     HOTG_Foundation
-    HOTG_Mem_Transitive_Closed
+    HOTG_Mem_Transitive_Closed_Base
+    Transport.Binary_Relations_Least
 begin
 
 paragraph \<open>Summary\<close>
@@ -14,61 +15,34 @@ In particular, each such set is transitively closed.
 
 We follow the approach from \<^cite>\<open>ZFC_in_HOL_AFP\<close>.\<close>
 
-definition "is_mem_trans_closure_of X T
-  \<equiv> mem_trans_closed T \<and> X \<subseteq> T \<and> (\<forall>Y : mem_trans_closed. X \<subseteq> Y \<longrightarrow> T \<subseteq> Y)"
+definition "mem_trans_closure X = least_wrt_rel (\<subseteq>) ((\<subseteq>) X \<sqinter> mem_trans_closed)"
 
-definition "mem_trans_closure X = (THE T. is_mem_trans_closure_of X T)"
-
-lemma is_mem_trans_closure_ofI:
-  assumes "mem_trans_closed T" "X \<subseteq> T" "\<And>Y. mem_trans_closed Y \<Longrightarrow> X \<subseteq> Y \<Longrightarrow> T \<subseteq> Y"
-  shows "is_mem_trans_closure_of X T"
-  using assms unfolding is_mem_trans_closure_of_def by blast
-
-lemma is_mem_trans_closure_ofE:
-  assumes "is_mem_trans_closure_of X T"
-  shows "mem_trans_closed T" "X \<subseteq> T" "\<And>Y. mem_trans_closed Y \<Longrightarrow> X \<subseteq> Y \<Longrightarrow> T \<subseteq> Y"
-  using assms unfolding is_mem_trans_closure_of_def by auto
-
-lemma eq_mem_trans_closure_if_is_mem_trans_closure_of:
-  assumes "is_mem_trans_closure_of X T"
-  shows "T = mem_trans_closure X"
-proof -
-  have "T = \<TT>" if "is_mem_trans_closure_of X \<TT>" for \<TT>
-    using assms that by (force elim: is_mem_trans_closure_ofE)
-  then have "\<exists>!T. is_mem_trans_closure_of X T" using assms by blast
-  from the1_equality[OF this] show ?thesis using assms mem_trans_closure_def by auto
-qed
-
-corollary is_mem_trans_closure_of_mem_trans_closure_if_is_mem_trans_closure_of:
-  assumes "is_mem_trans_closure_of X T"
-  shows "is_mem_trans_closure_of X (mem_trans_closure X)"
-  using assms eq_mem_trans_closure_if_is_mem_trans_closure_of by blast
-
-lemma has_mem_trans_closure_if_elements_have:
-  assumes trans_closure_elems: "\<And>x. x \<in> X \<Longrightarrow> is_mem_trans_closure_of x (mem_trans_closure x)"
+lemma is_least_wrt_rel_mem_trans_closed_if_mem_is_least_wrt_rel_mem_trans_closed:
+  assumes trans_closure_elems:
+    "\<And>x. x \<in> X \<Longrightarrow> is_least_wrt_rel (\<subseteq>) ((\<subseteq>) x \<sqinter> mem_trans_closed) (mem_trans_closure x)"
   defines "T \<equiv> X \<union> (\<Union>x \<in> X. mem_trans_closure x)"
-  shows "is_mem_trans_closure_of X T"
-proof (intro is_mem_trans_closure_ofI)
+  shows "is_least_wrt_rel (\<subseteq>) ((\<subseteq>) X \<sqinter> mem_trans_closed) T"
+proof (intro is_least_wrt_rel_if_antisymmetric_onI is_minimal_wrt_relI inf1I)
   show "mem_trans_closed T"
   proof (intro mem_trans_closedI)
     fix z assume "z \<in> T"
-    then consider (mem) "z \<in> X" | (trans) x where "x \<in> X" "z \<in> mem_trans_closure x" using T_def by auto
+    then consider (mem) "z \<in> X" | (step) x where "x \<in> X" "z \<in> mem_trans_closure x"
+      using T_def by auto
     then show "z \<subseteq> T"
     proof cases
       case mem
-      then have "z \<subseteq> mem_trans_closure z"
-        using trans_closure_elems is_mem_trans_closure_ofE mem_trans_closedD by auto
+      then have "z \<subseteq> mem_trans_closure z" using trans_closure_elems by auto
       then show ?thesis using \<open>z \<in> X\<close> T_def by auto
     next
-      case trans
+      case step
       then have "z \<subseteq> mem_trans_closure x"
-        using trans_closure_elems is_mem_trans_closure_ofE mem_trans_closedD by auto
+        using trans_closure_elems mem_trans_closedD by (blast elim!: is_least_wrt_relE)
       then show ?thesis using \<open>x \<in> X\<close> T_def by auto
     qed
   qed
 next show "X \<subseteq> T" unfolding T_def by auto
 next
-  fix Y assume hY: "mem_trans_closed Y" "X \<subseteq> Y"
+  fix Y presume hY: "mem_trans_closed Y" "X \<subseteq> Y"
   show "T \<subseteq> Y"
   proof
     fix z assume "z \<in> T"
@@ -80,27 +54,27 @@ next
     next
       case trans
       then have "mem_trans_closure x \<subseteq> Y"
-        using trans_closure_elems is_mem_trans_closure_ofE hY by blast
+        using trans_closure_elems hY by (blast elim!: is_least_wrt_relE)
       then show ?thesis using trans by auto
     qed
   qed
-qed
+qed auto
 
-theorem is_mem_trans_closure_of_mem_trans_closure:
-  shows "is_mem_trans_closure_of X (mem_trans_closure X)"
+theorem is_least_wrt_rel_mem_trans_closure:
+  "is_least_wrt_rel (\<subseteq>) ((\<subseteq>) X \<sqinter> mem_trans_closed) (mem_trans_closure X)"
 proof (induction X rule: mem_induction)
   case (mem X)
-  then show ?case using has_mem_trans_closure_if_elements_have
-    using is_mem_trans_closure_of_mem_trans_closure_if_is_mem_trans_closure_of by blast
+  then show ?case by (subst mem_trans_closure_def, subst least_wrt_rel_eqI)
+    (rule is_least_wrt_rel_mem_trans_closed_if_mem_is_least_wrt_rel_mem_trans_closed)
 qed
 
 corollary mem_trans_closure_eq_bin_union_idx_union:
   "mem_trans_closure X = X \<union> (\<Union>x \<in> X. mem_trans_closure x)"
-  using has_mem_trans_closure_if_elements_have is_mem_trans_closure_of_mem_trans_closure
-  using eq_mem_trans_closure_if_is_mem_trans_closure_of[symmetric] by auto
+  using is_least_wrt_rel_mem_trans_closure by (subst mem_trans_closure_def, subst least_wrt_rel_eqI)
+  (auto intro: is_least_wrt_rel_mem_trans_closed_if_mem_is_least_wrt_rel_mem_trans_closed)
 
 corollary subset_mem_trans_closure_self: "X \<subseteq> mem_trans_closure X"
-  using is_mem_trans_closure_of_mem_trans_closure is_mem_trans_closure_ofE by auto
+  using mem_trans_closure_eq_bin_union_idx_union by blast
 
 corollary mem_mem_trans_closure_if_mem: "X \<in> Y \<Longrightarrow> X \<in> mem_trans_closure Y"
   using subset_mem_trans_closure_self by blast
@@ -126,7 +100,7 @@ lemma mem_trans_closure_eq_empty_iff_eq_empty [iff]: "mem_trans_closure X = {} \
   using subset_mem_trans_closure_self by auto
 
 lemma mem_trans_closed_mem_trans_closure: "mem_trans_closed (mem_trans_closure X)"
-  using is_mem_trans_closure_of_mem_trans_closure is_mem_trans_closure_ofE by auto
+  using is_least_wrt_rel_mem_trans_closure by auto
 
 lemma not_mem_mem_trans_closure_self [iff]: "X \<notin> mem_trans_closure X"
 proof
@@ -140,7 +114,7 @@ qed
 
 lemma mem_trans_closure_le_if_le_if_mem_trans_closed:
   "mem_trans_closed X \<Longrightarrow> Y \<subseteq> X \<Longrightarrow> mem_trans_closure Y \<subseteq> X"
-  using is_mem_trans_closure_of_mem_trans_closure is_mem_trans_closure_ofE(3) by blast
+  using is_least_wrt_rel_mem_trans_closure by blast
 
 lemma mem_trans_closure_subset_mem_trans_closure_if_subset:
   assumes "Y \<subseteq> X"
