HOTG/Arithmetics/HOTG_Arithmetics_Cardinal_Arithmetics.thy
@@ -3,10 +3,10 @@
 subsection \<open>Compatibility of Set Arithmetics and Cardinal Arithmetics\<close>
 theory HOTG_Arithmetics_Cardinal_Arithmetics
   imports
+    HOTG_Bounded_Definite_Description
     HOTG_Cardinals_Addition
     HOTG_Cardinals_Multiplication
     HOTG_Addition
-    HOTG_Functions_Injective
     HOTG_Multiplication
 begin
 
@@ -24,14 +24,15 @@ qed
 
 text\<open>The next theorem shows that set addition is compatible with cardinality addition.\<close>
 
-(*TODO: cardinalities on rhs can be removed*)
-theorem cardinality_add_eq_cardinal_add_cardinality: "|X + Y| = |X| \<oplus> |Y|"
-  using disjoint_lift_self_right by (auto simp add:
-  cardinality_bin_union_eq_cardinal_add_cardinality_if_disjoint add_eq_bin_union_lift)
+theorem cardinality_add_eq_cardinal_add: "|X + Y| = X \<oplus> Y"
+  unfolding add_eq_bin_union_lift
+  by (subst cardinality_bin_union_eq_cardinal_add_if_disjoint[OF disjoint_lift_self_right],
+    subst cardinality_cardinal_add_eq_cardinal_add[symmetric])
+  (simp add: cardinality_lift_eq_cardinality_right)
 
 text\<open>The next theorems show that set multiplication is compatible with cardinality multiplication.\<close>
 
-theorem cardinality_mul_eq_cardinal_pair: "|X * Y| = |X \<times> Y|"
+lemma mul_equipollent_pair: "X * Y \<approx> X \<times> Y"
 proof -
   define f :: "set \<Rightarrow> set" where "f \<equiv> \<lambda>\<langle>x, y\<rangle>. X * y + x"
   have "injective_on (X \<times> Y :: set) f"
@@ -45,15 +46,15 @@ proof -
     then show "p\<^sub>1 = p\<^sub>2" using \<open>p\<^sub>1 = \<langle>x\<^sub>1, y\<^sub>1\<rangle>\<close> \<open>p\<^sub>2 = \<langle>x\<^sub>2, y\<^sub>2\<rangle>\<close> by auto
   qed auto
   then obtain g where "bijection_on (X \<times> Y) (image f (X \<times> Y)) f g"
-    using bijection_on_image_if_injective_on by blast
-  then have "X \<times> Y \<approx> image f (X \<times> Y)" using equipollentI by blast
+    using bijection_on_image_the_inverse_on_if_injective_on by blast
   moreover have "image f (X \<times> Y) = X * Y"
-    unfolding mul_eq_idx_union_repl_mul_add[of X Y] f_def by force
-  ultimately show ?thesis using cardinality_eq_if_equipollent by auto
+    unfolding mul_eq_idx_union_repl_mul_add[of X Y] f_def by fastforce
+  ultimately show ?thesis by (intro equipollentI) fastforce
 qed
 
 theorem cardinality_mul_eq_cardinal_mul: "|X * Y| = X \<otimes> Y"
-  using cardinality_mul_eq_cardinal_pair cardinal_mul_eq_cardinality_pair by simp
+  unfolding cardinal_mul_eq_cardinality_pair
+  by (intro cardinality_eq_if_equipollent mul_equipollent_pair)
 
 end
 
