HOTG/Orders/HOTG_Orders.thy
@@ -1,9 +1,8 @@
 \<^marker>\<open>creator "Kevin Kappelmann"\<close>
 theory HOTG_Orders
   imports
-    HOTG_Less_Than
-    HOTG_Well_Orders
     HOTG_Additively_Divides
+    HOTG_Less_Than
 begin
 
 
